\input{mmd6-article-leader}
\def\mytitle{Math}
\input{mmd6-article-begin}

foo \({e}^{i\pi }+1=0\) bar

\[ {x}_{1,2}=\frac{-b\pm \sqrt{{b}^{2}-4ac}}{2a} \]

foo ${e}^{i\pi }+1=0$ bar

foo ${e}^{i\pi }+1=0$, bar

$${x}_{1,2}=\frac{-b\pm \sqrt{{b}^{2}-4ac}}{2a}$$

5

foo \$ \{e\}\^{}\{i\textbackslash{}pi \}+1=0\$ bar

\$\$ \{x\}\_\{1,2\}=\textbackslash{}frac\{-b\textbackslash{}pm \textbackslash{}sqrt\{\{b\}\^{}\{2\}-4ac\}\}\{2a\}\$\$

foo \$\{e\}\^{}\{i\textbackslash{}pi \}+1=0 \$ bar

\$\$\{x\}\_\{1,2\}=\textbackslash{}frac\{-b\textbackslash{}pm \textbackslash{}sqrt\{\{b\}\^{}\{2\}-4ac\}\}\{2a\} \$\$

foo a\$\{e\}\^{}\{i\textbackslash{}pi \}+1=0\$ bar

10

a\$\$\{x\}\_\{1,2\}=\textbackslash{}frac\{-b\textbackslash{}pm \textbackslash{}sqrt\{\{b\}\^{}\{2\}-4ac\}\}\{2a\}\$\$

foo \$\{e\}\^{}\{i\textbackslash{}pi \}+1=0\$b bar

\$\$\{x\}\_\{1,2\}=\textbackslash{}frac\{-b\textbackslash{}pm \textbackslash{}sqrt\{\{b\}\^{}\{2\}-4ac\}\}\{2a\}\$\$b

$\nabla \times \mathbf{E} = - \frac{\partial \mathbf{B}}{\partial t}$

$$\nabla \times \mathbf{E} = - \frac{\partial \mathbf{B}}{\partial t}$$

15

\(\nabla \times \mathbf{E} = - \frac{\partial \mathbf{B}}{\partial t}\)

\[\nabla \times \mathbf{E} = - \frac{\partial \mathbf{B}}{\partial t}\]

\begin{equation}\nabla \times \mathbf{E} = - \frac{\partial \mathbf{B}}{\partial t}\end{equation}

\begin{equation}\nabla \times \mathbf{E} = - \frac{\partial \mathbf{B}}{\partial t}\end{equation}

\begin{equation}\nabla \times \mathbf{E} = - \frac{\partial \mathbf{B}}{\partial t}\end{equation}

20

\begin{equation}\nabla \times \mathbf{E} = - \frac{\partial \mathbf{B}}{\partial t}\end{equation}

\texttt{\textbackslash{}begin\{equation\}\textbackslash{}nabla \textbackslash{}times \textbackslash{}mathbf\{E\} = - \textbackslash{}frac\{\textbackslash{}partial \textbackslash{}mathbf\{B\}\}\{\textbackslash{}partial t\}\textbackslash{}end\{equation\}}

$a *foo* b$

\[a *foo* b\]

\input{mmd6-article-footer}
\end{document}
